# Section 5.5

In this section we will look at solving nonlinear system of equations.

::::{prf:example}
:label: nonLinearSystem1

Solve the system

$$
\begin{cases}
x^{2}-y & =4\\
x+y & =-2
\end{cases}
$$

:::{dropdown} Solution:

Notice this is not a system of linear equations. However, we can simply rewrite the system as follows 

$$
\begin{cases}
x^{2}-y & =4\\
x+y & =-2
\end{cases}\to\begin{cases}
y & =x^{2}-4\\
y & =-x-2
\end{cases}
$$

and notice that 

$$
y=y\iff x^{2}-4=-x-2
$$

Solving

\begin{align*}
x^{2}-4 & =-x-2\\
x^{2}+x-4+2 & =0\\
x^{2}+x-2 & =0\\
(x+2)(x-1) & =0
\end{align*}

we have $x=-2$ and $x=1$.

When $x=-2$ we have

$$
-2+y=-2\iff y=0
$$

When $x=1$ we have

$$
1+y=-2\iff y=-3.
$$

Therefore, the solution set for the system is $\{(-2,0),(1,-3)\}$.

:::
::::

::::{prf:example}
:label: nonLinearSystem2

Solve the system

$$
\begin{cases}
x^{2}+y^{2} & =9\\
9x^{2}+4y^{2} & =36
\end{cases}
$$

:::{dropdown} Solution:

Here we will use the elimination method to solve for $y$

\begin{align*}
\begin{cases}
x^{2}+y^{2} & =9\\
9x^{2}+4y^{2} & =36
\end{cases} & \to\begin{cases}
9x^{2}+9y^{2} & =81\\
9x^{2}+4y^{2} & =36
\end{cases}\\
 & \to5y^{2}=45\\
 & \to y^{2}=9\\
 & \to y=\pm3
\end{align*}

When $y=3$ we have

\begin{align*}
x^{2}+(3)^{3} & =9\\
x^{2}+9 & =9\\
x^{2} & =0\implies x=0
\end{align*}

When $y=-3$ we have

\begin{align*}
x^{2}+(-3)^{2} & =9\\
x^{2}+9 & =0\\
x^{2} & =0\implies x=0
\end{align*}

Therefore, the solution set for the system is $\{(0,3),(0,-3)\}$.

:::
::::


::::{prf:example}
:label: nonLinearSystem3

Solve the system

$$
\begin{cases}
x^{2}+xy+y^{2} & =21\\
x^{2}-xy+y^{2} & =9
\end{cases}
$$

:::{dropdown} Solution:

If use the elimination method we have

\begin{align*}
\begin{cases}
x^{2}+xy+y^{2} & =21\\
x^{2}-xy+y^{2} & =9
\end{cases} & \to2x^{2}+2y^{2}=30\\
 & \to x^{2}+y^{2}=15\\
 & \to\begin{cases}
y^{2} & =15-x^{2}\\
y & =\pm\sqrt{15-x^{2}}
\end{cases}
\end{align*}

---

When $y=15-x^{2}$ and $y=\sqrt{15-x^{2}}$

\begin{align*}
x^{2}+x\sqrt{15-x^{2}}+15-x^{2} & =21\\
x\sqrt{15-x^{2}}+15 & =21\\
x\sqrt{15-x^{2}} & =6\\
\sqrt{15-x^{2}} & =\frac{6}{x}\\
15-x^{2} & =\frac{36}{x^{2}}\\
15x^{2}-x^{4} & =36\\
x^{4}-15x^{2}+36 & =0\\
(x^{2}-12)(x^{2}-3) & =0\\
x^{2} & =12\implies x=\pm\sqrt{12}=\pm2\sqrt{3}\\
x^{2} & =3\implies x=\pm\sqrt{3}
\end{align*}

When we go back to 

\begin{align*}
x^{2}+x\sqrt{15-x^{2}}+15-x^{2} & =21\\
x\sqrt{15-x^{2}}+15 & =21\\
x\sqrt{15-x^{2}} & =6
\end{align*}

We see that $x\ne-\sqrt{3}$ and $x\ne-2\sqrt{3}$ (check on your own). Therefore, $x=\sqrt{3}$ or $x=2\sqrt{3}$.

When $x=\sqrt{3}$ we have $y=\sqrt{15-(\sqrt{3})^{2}}=2\sqrt{3}$.

When $x=2\sqrt{3}$ we have $y=\sqrt{15-(2\sqrt{3})^{2}}=\sqrt{3}$. Therefore, two elements in the solution set is $\{(\sqrt{3},2\sqrt{3}),(2\sqrt{3},\sqrt{3})\}$.

---

When $y^{2}=15-x^{2}$ and $y=-\sqrt{15-x^{2}}$ we have

\begin{align*}
x^{2}-x\sqrt{15-x^{2}}+15-x^{2} & =21\\
-x\sqrt{15-x^{2}}+15 & =21\\
-x\sqrt{15-x^{2}} & =6\\
\sqrt{15-x^{2}} & =-\frac{6}{x}\\
15-x^{2} & =\frac{36}{x^{2}}\\
15x^{2}-x^{4} & =36\\
x^{4}-15x+36 & =0
\end{align*}

which we already know the solution to, $\{\pm\sqrt{3},\pm2\sqrt{3}\}$.

However, when we look at

\begin{align*}
x^{2}-x\sqrt{15-x^{2}}+15-x^{2} & =21\\
-x\sqrt{15-x^{2}}+15 & =21\\
-x\sqrt{15-x^{2}} & =6
\end{align*}

we see that $x\ne\sqrt{3}$ and $x\ne2\sqrt{3}$ (check on your own). Therefore, $x=-\sqrt{3}$ and $x=-2\sqrt{3}$.

When $x=-\sqrt{3}$ we have $y=-\sqrt{15-(-\sqrt{3})^{2}}=-2\sqrt{3}$.

When $x=-2\sqrt{3}$ we have $y=-\sqrt{15-(-2\sqrt{3})^{2}}=-\sqrt{3}$.

This then added $(-\sqrt{3},-2\sqrt{3})$ and $(-2\sqrt{3},-\sqrt{3})$ to the solution set.

---

Therefore, the solution set is 

$$
\{(\sqrt{3},2\sqrt{3}),(2\sqrt{3},\sqrt{3}),(-\sqrt{3},-2\sqrt{3}),(-2\sqrt{3},-\sqrt{3})\}
$$

:::
::::

