# Section 7.3

:::{prf:definition} Geometric Sequence
:label: geoSeqDef

A geometric sequence is a sequence in which each term after the first is obtained by multiplying the preceding term by a fixed nonzero real number, called the **common ratio**.

We find the common ratio by choosing any term after the first and dividing it by the preceding term.

In a geometric sequence with first term $a_{1}$ and common ratio $r$, the $n$th term $a_{n}$ is given by the following

$$
a_{n}=a_{1}r^{n-1}.
$$
:::

Something to keep in mind when dealing with geometric sequences. The first value, $a_1$, is your starting number and by definition is $a_1=a_1\cdot r^0=a_1$. Then the next number in the sequence is $a_2$ which is $a_1$ times $r$. That is,

$$a_2=a_1\cdot r$$

The next number is $a_3$ which is $a_2$ times $r$. That is,

\begin{align*}
    a_3 & = a_2\cdot r\\ 
    & = \left(a_1 \cdot r \right)\cdot r\\
    & = a_1\cdot r^2
\end{align*}

The next number is $a_4$ which is $a_3$ times $r$. That is,

\begin{align*}
    a_4 & = a_3\cdot r\\
    & = \left(a_2\cdot r\right)\cdot r\\
    & = \left(\left(a_1\cdot r\right)\cdot r\right)\cdot r\\
    & = a_1\cdot r^3
\end{align*}

And so on. This commonly associated with compound interest.

::::{prf:example}
:label: geoSeqExam1

Determine $a_{5}$ and $a_{n}$for the geometric sequence

$$
6400,\,1600,\,400,\,100,\,...
$$

:::{dropdown} Solution:

First,

$$
\frac{1600}{6400}=\frac{1}{4}=r
$$

and $a_{1}=6400$. Therefore, $a_{n}=6400\cdot4^{n-1}$. Thus,

\begin{align*}
a_{5} & =6400\cdot(\frac{1}{4})^{5-1}\\
 & =6400\cdot\left(\frac{1}{4}\right)^{4}\\
 & =25
\end{align*}

or since $a_{4}=100$ we know that $a_{5}=100\div4=25$.
:::
::::

::::{prf:example}
:label: geoSeqExam2

Determine $r$ and $a_{1}$ for the geometric sequence with $a_{2}=-18$ and $a_{5}=486$. Then define $a_{n}$.

:::{dropdown} Solution:

Consider a table of values

\begin{align*}
a_{1} & =a_{1}r^{0}=a_1\\
a_{2} & =a_{1}r=-18\\
a_{3} & =a_{2}\cdot r=-18\cdot r\\
a_{4} & =a_{3}\cdot r=\left(a_{2}\cdot r\right)\cdot r=a_{2}r^{2}=-18r^{2}\\
a_{5} & =a_{4}\cdot r=\left(-18r^{2}\right)\cdot r=-18r^{3}=486
\end{align*}

Thus, we can solve for $r$

\begin{align*}
-18r^{3} & =486\\
r^{3} & =\frac{486}{-18}\\
 & =-27\\
r & =-3
\end{align*}
Since $a_{2}=a_{1}r^{2-1}$ we have
\begin{align*}
-18 & =a_{1}(-3)^{1}\\
-18 & =a_{1}(-3)\\
a_{1} & =\frac{-18}{-3}\\
 & =6
\end{align*}

Therefore, $a_{1}=6$, $r=-3$ and $a_{n}=6(-3)^{n-1}$.

:::
::::