# Section 4.1

$$a\times n=\underset{n\text{ amount of times}}{\underbrace{a+a+\,\dots\,+a}}$$

$$a^{n}=\underset{n\text{ amount of times}}{\underbrace{a\cdot a\cdot\,\dots\,\cdot a}}$$

$$a^{n}\cdot a^{m}=\underset{n+m\text{ amount of times}}{\underbrace{\left(\underset{n\text{ amount of times}}{\underbrace{a\cdot a\cdot\,\dots\,\cdot a}}\right)\cdot\left(\underset{m\text{ amount of times}}{\underbrace{a\cdot a\cdot\,\dots\,\cdot a}}\right)}}=a^{m+n}$$

\begin{align*}
\left(a^{m}\right)^{n} & =a^{m}\cdot a^{m}\cdot\,\dots\,\cdot a^{m}\\
 & =\underset{m+m+\dots+m=nm\text{ amount of times}}{\underbrace{\left(\underset{m\text{ amount of times}}{\underbrace{a\cdot a\cdot\,\dots\,\cdot a}}\right)\cdot\left(\underset{m\text{ amount of times}}{\underbrace{a\cdot a\cdot\,\dots\,\cdot a}}\right)\cdot\,\dots\,\cdot\left(\underset{m\text{ amount of times}}{\underbrace{a\cdot a\cdot\,\dots\,\cdot a}}\right)}}\\
 & =a^{nm}
\end{align*}

![demo neg exponent](images/negExp.png)